Refactor auxiliary definitions

RegexCorrectness/VM/CharStep/Lemmas.lean
@@ -14,14 +14,12 @@ namespace Regex.VM
 
 variable {nfa : NFA} {wf : nfa.WellFormed} {it : Iterator}
   {current : SearchState' nfa} {currentUpdates : Vec (List (Nat × Pos)) nfa.nodes.size}
-  {next : SparseSet nfa.nodes.size} {updates : Vec (List (Nat × String.Pos)) nfa.nodes.size}
-  {state : Fin nfa.nodes.size}
-  {next' : SparseSet nfa.nodes.size} {matched' : Option (List (Nat × Pos))}
-  {updates' : Vec (List (Nat × String.Pos)) nfa.nodes.size}
+  {next : SearchState' nfa} {state : Fin nfa.nodes.size}
+  {matched' : Option (List (Nat × Pos))} {next' : SearchState' nfa}
 
-theorem stepChar.lower_bound (h : stepChar' nfa wf it currentUpdates next updates state = (next', matched', updates'))
-  (lb : εClosure.LowerBound next) :
-  εClosure.LowerBound next' := by
+theorem stepChar.lower_bound (h : stepChar' nfa wf it currentUpdates next state = (matched', next'))
+  (lb : εClosure.LowerBound next.states) :
+  εClosure.LowerBound next'.states := by
   simp [stepChar'] at h
   split at h
   next c' state' hn =>
@@ -34,9 +32,9 @@ theorem stepChar.lower_bound (h : stepChar' nfa wf it currentUpdates next update
     next => simp_all
   next => simp_all
 
-theorem stepChar.eq_updates_of_mem_next {i k} (h : stepChar' nfa wf it currentUpdates next updates i = (next', matched', updates'))
-  (mem : k ∈ next) :
-  updates'[k] = updates[k] := by
+theorem stepChar.eq_updates_of_mem_next {i k} (h : stepChar' nfa wf it currentUpdates next i = (matched', next'))
+  (mem : k ∈ next.states) :
+  next'.updates[k] = next.updates[k] := by
   simp [stepChar'] at h
   split at h
   next c' j hn =>
@@ -50,10 +48,10 @@ theorem stepChar.eq_updates_of_mem_next {i k} (h : stepChar' nfa wf it currentUp
   next => simp_all
 
 theorem mem_next_of_stepChar {l m r i j k update}
-  (h : stepChar' nfa wf it currentUpdates next updates i = (next', matched', updates'))
-  (lb : εClosure.LowerBound next)
+  (h : stepChar' nfa wf it currentUpdates next i = (matched', next'))
+  (lb : εClosure.LowerBound next.states)
   (step : nfa.CharStep l m it.curr r i j) (cls : nfa.εClosure' ⟨l, it.curr :: m, r⟩ j k update) :
-  k ∈ next' := by
+  k ∈ next'.states := by
   simp [stepChar'] at h
   split at h
   next c' j' hn =>
@@ -69,13 +67,13 @@ theorem mem_next_of_stepChar {l m r i j k update}
     simp_all
 
 theorem write_updates_of_mem_next_of_stepChar {i k} (span : Span) (hspan : span.iterator = it)
-  (h : stepChar' nfa wf it currentUpdates next updates i = (next', matched', updates'))
-  (notEnd : ¬it.atEnd) (mem : k ∈ next') :
-  k ∈ next ∨ ∃ r' j update',
+  (h : stepChar' nfa wf it currentUpdates next i = (matched', next'))
+  (notEnd : ¬it.atEnd) (mem : k ∈ next'.states) :
+  k ∈ next.states ∨ ∃ r' j update',
     span.r = it.curr :: r' ∧
     nfa.CharStep span.l span.m it.curr r' i j ∧
     nfa.εClosure' span.next j k update' ∧
-    (WriteUpdate k → updates'[k] = currentUpdates.get i i.isLt ++ update') := by
+    (WriteUpdate k → next'.updates[k] = currentUpdates.get i i.isLt ++ update') := by
   simp [stepChar'] at h
   split at h
   next c j hn =>
@@ -104,33 +102,36 @@ theorem write_updates_of_mem_next_of_stepChar {i k} (span : Span) (hspan : span.
     next => simp_all only [SparseSet.mem_mem, Prod.mk.injEq, exists_and_left, true_or]
   next => simp_all only [SparseSet.mem_mem, Prod.mk.injEq, exists_and_left, true_or]
 
-theorem eachStepChar.go.lower_bound {i hle} (h : eachStepChar'.go nfa wf it current i hle next updates = (next', matched', updates'))
-  (lb : εClosure.LowerBound next) :
-  εClosure.LowerBound next' := by
-  induction i, hle, next, updates using eachStepChar'.go.induct' nfa wf it current with
-  | base next updates => simp_all
-  | found i next updates hlt next'' matched updates' h' found =>
+theorem eachStepChar.go.lower_bound {i hle} (h : eachStepChar'.go nfa wf it current i hle next = (matched', next'))
+  (lb : εClosure.LowerBound next.states) :
+  εClosure.LowerBound next'.states := by
+  induction i, hle, next using eachStepChar'.go.induct' nfa wf it current with
+  | base next => simp_all
+  | found i hlt next matched next'' h' found =>
     rw [eachStepChar'.go_found hlt h' found] at h
     simp_all
     exact stepChar.lower_bound h' lb
-  | not_found i next updates hlt next'' matched updates' h' not_found ih =>
+  | not_found i hlt next matched next'' h' not_found ih =>
     rw [eachStepChar'.go_not_found hlt h' not_found] at h
     exact ih h (stepChar.lower_bound h' lb)
 
-def eachStepChar.Inv (nfa : NFA) (wf : nfa.WellFormed) (it : Iterator)
-  (next : SparseSet nfa.nodes.size) (updates : Vec (List (Nat × Pos)) nfa.nodes.size) : Prop :=
-  ∀ i ∈ next, ∃ span update, span.iterator = it ∧ nfa.VMPath wf span i update ∧ (WriteUpdate i → updates[i] = update)
+def eachStepChar.Inv (nfa : NFA) (wf : nfa.WellFormed) (it : Iterator) (next : SearchState' nfa) : Prop :=
+  ∀ i ∈ next.states,
+    ∃ span update,
+      span.iterator = it ∧
+      nfa.VMPath wf span i update ∧
+      (WriteUpdate i → next.updates[i] = update)
 
-theorem eachStepChar.Inv.of_empty (h : next.isEmpty) : eachStepChar.Inv nfa wf it next updates := by
+theorem eachStepChar.Inv.of_empty (h : next.states.isEmpty) : eachStepChar.Inv nfa wf it next := by
   intro i mem
   exact (SparseSet.not_mem_of_isEmpty h mem).elim
 
 theorem eachStepChar.Inv.of_stepChar {idx} (hlt : idx < current.states.count)
-  (h : stepChar' nfa wf it current.updates next updates current.states[idx] = (next', matched', updates'))
+  (h : stepChar' nfa wf it current.updates next current.states[idx] = (matched', next'))
   (notEnd : ¬it.atEnd)
-  (inv_curr : eachStepChar.Inv nfa wf it current.states current.updates)
-  (inv_next : eachStepChar.Inv nfa wf it.next next updates) :
-  eachStepChar.Inv nfa wf it.next next' updates' := by
+  (inv_curr : eachStepChar.Inv nfa wf it current)
+  (inv_next : eachStepChar.Inv nfa wf it.next next) :
+  eachStepChar.Inv nfa wf it.next next' := by
   have ⟨span, update, eqit, path, write⟩ := inv_curr current.states[idx] (SparseSet.mem_get hlt)
 
   intro k mem
@@ -142,36 +143,31 @@ theorem eachStepChar.Inv.of_stepChar {idx} (hlt : idx < current.states.count)
     exact equ ▸ inv
   | .inr ⟨r', j, update', eqr, step, cls, write'⟩ =>
     simp [step.write_update] at write
-    have write'' : WriteUpdate k → updates'[k] = update ++ update' := write ▸ write'
+    have write'' : WriteUpdate k → next'.updates[k] = update ++ update' := write ▸ write'
     exact ⟨span.next, update ++ update', by rw [Span.next_iterator eqr, eqit], .more path eqr step cls, write''⟩
 
-theorem eachStepChar.go.inv {idx hle} (h : eachStepChar'.go nfa wf it current idx hle next updates = (next', matched', updates'))
+theorem eachStepChar.go.inv {idx hle} (h : eachStepChar'.go nfa wf it current idx hle next = (matched', next'))
   (notEnd : ¬it.atEnd)
-  (inv_curr : eachStepChar.Inv nfa wf it current.states current.updates)
-  (inv_next : eachStepChar.Inv nfa wf it.next next updates) :
-  eachStepChar.Inv nfa wf it.next next' updates' := by
-  induction idx, hle, next, updates using eachStepChar'.go.induct' nfa wf it current with
-  | base next updates => simp_all
-  | found idx next updates hlt next'' matched updates'' h' found =>
+  (inv_curr : eachStepChar.Inv nfa wf it current)
+  (inv_next : eachStepChar.Inv nfa wf it.next next) :
+  eachStepChar.Inv nfa wf it.next next' := by
+  induction idx, hle, next using eachStepChar'.go.induct' nfa wf it current with
+  | base next => simp_all
+  | found idx hlt next matched next'' h' found =>
     rw [eachStepChar'.go_found hlt h' found] at h
     simp_all
     exact eachStepChar.Inv.of_stepChar hlt h' (by simp [notEnd]) inv_curr inv_next
-  | not_found idx next updates hlt next'' matched updates'' h' not_found ih =>
+  | not_found idx hlt next matched next'' h' not_found ih =>
     rw [eachStepChar'.go_not_found hlt h' not_found] at h
-    have inv' : eachStepChar.Inv nfa wf it.next next'' updates'' :=
+    have inv' : eachStepChar.Inv nfa wf it.next next'' :=
       eachStepChar.Inv.of_stepChar hlt h' (by simp [notEnd]) inv_curr inv_next
     apply ih h inv'
 
-theorem eachStepChar.inv {next next'} (h : eachStepChar' nfa wf it current next = (next', matched'))
+theorem eachStepChar.inv {next next'} (h : eachStepChar' nfa wf it current next = (matched', next'))
   (notEnd : ¬it.atEnd) (empty : next.states.isEmpty)
-  (inv : eachStepChar.Inv nfa wf it current.states current.updates) :
-  eachStepChar.Inv nfa wf it.next next'.states next'.updates := by
+  (inv : eachStepChar.Inv nfa wf it current) :
+  eachStepChar.Inv nfa wf it.next next' := by
   simp [eachStepChar'] at h
-  set result := eachStepChar'.go nfa wf it current 0 (Nat.zero_le _) next.states next.updates
-  set nextStates := result.1
-  set nextUpdates := result.2.2
-  have : result = (nextStates, matched', nextUpdates) := by
-    simp [←h]
-  exact h.1 ▸ eachStepChar.go.inv this notEnd inv (eachStepChar.Inv.of_empty empty)
+  exact eachStepChar.go.inv h notEnd inv (eachStepChar.Inv.of_empty empty)
 
 end Regex.VM
