RegexCorrectness/VM/EpsilonClosure/Basic.lean
@@ -2,6 +2,7 @@ import Regex.Data.Array
 import Regex.Data.SparseSet
 import Regex.NFA.Basic
 import Regex.VM
+import RegexCorrectness.VM.Basic2
 
 set_option autoImplicit false
 
@@ -21,118 +22,123 @@ As the NFA semantics use `List (Nat × Pos)` to represent the capture group upda
 updates as a `Buffer` for efficiency, and the correspondence will be proved in `Correspondence.lean`.
 -/
 def εClosure' (nfa : NFA) (wf : nfa.WellFormed) (it : Iterator)
-  (next : SparseSet nfa.nodes.size) (matched : Option (List (Nat × Pos))) (updates : Vec (List (Nat × Pos)) nfa.nodes.size)
-  (stack : εStack' nfa) :
-  (SparseSet nfa.nodes.size × Option (List (Nat × Pos)) × Vec (List (Nat × Pos)) nfa.nodes.size) :=
+  (matched : Option (List (Nat × Pos))) (next : SearchState' nfa) (stack : εStack' nfa) :
+  Option (List (Nat × Pos)) × SearchState' nfa :=
   match stack with
-  | [] => (next, matched, updates)
+  | [] => (matched, next)
   | (update, state) :: stack' =>
-    if state ∈ next then
-      εClosure' nfa wf it next matched updates stack'
+    if state ∈ next.states then
+      εClosure' nfa wf it matched next stack'
     else
-      let next' := next.insert state
+      let states' := next.states.insert state
       match hn : nfa[state] with
       | .epsilon state' =>
         have isLt : state' < nfa.nodes.size := wf.inBounds' state hn
-        εClosure' nfa wf it next' matched updates ((update, ⟨state', isLt⟩) :: stack')
+        εClosure' nfa wf it matched ⟨states', next.updates⟩ ((update, ⟨state', isLt⟩) :: stack')
       | .split state₁ state₂ =>
         have isLt : state₁ < nfa.nodes.size ∧ state₂ < nfa.nodes.size := wf.inBounds' state hn
-        εClosure' nfa wf it next' matched updates ((update, ⟨state₁, isLt.1⟩) :: (update, ⟨state₂, isLt.2⟩):: stack')
+        εClosure' nfa wf it matched ⟨states', next.updates⟩ ((update, ⟨state₁, isLt.1⟩) :: (update, ⟨state₂, isLt.2⟩):: stack')
       | .save offset state' =>
         have isLt : state' < nfa.nodes.size := wf.inBounds' state hn
         let update' := update ++ [(offset, it.pos)]
-        εClosure' nfa wf it next' matched updates ((update', ⟨state', isLt⟩) :: stack')
+        εClosure' nfa wf it matched ⟨states', next.updates⟩ ((update', ⟨state', isLt⟩) :: stack')
       | .done =>
         let matched' := matched <|> update
-        let buffers' := updates.set state state.isLt update
-        εClosure' nfa wf it next' matched' buffers' stack'
+        let updates' := next.updates.set state state.isLt update
+        εClosure' nfa wf it matched' ⟨ states', updates'⟩ stack'
       | .char c state' =>
-        let buffers' := updates.set state state.isLt update
-        εClosure' nfa wf it next' matched buffers' stack'
+        let updates' := next.updates.set state state.isLt update
+        εClosure' nfa wf it matched ⟨ states', updates'⟩ stack'
       | .sparse cs state' =>
-        let buffers' := updates.set state state.isLt update
-        εClosure' nfa wf it next' matched buffers' stack'
-      | .fail => εClosure' nfa wf it next' matched updates stack'
-termination_by (next.measure, stack)
+        let updates' := next.updates.set state state.isLt update
+        εClosure' nfa wf it matched ⟨ states', updates'⟩ stack'
+      | .fail => εClosure' nfa wf it matched ⟨states', next.updates⟩ stack'
+termination_by (next.states.measure, stack)
 
--- Tidied up version of the function induction
+-- Cleaner version of the fuction induction principle
+-- Using tactics in the body crashes Lean due to too high memory usage
 theorem εClosure'.induct' (nfa : NFA) (wf : nfa.WellFormed) (it : Iterator)
-  (motive : SparseSet nfa.nodes.size → Option (List (Nat × Pos)) → Vec (List (Nat × Pos)) nfa.nodes.size → εStack' nfa → Prop)
-  (base : ∀ next matched updates, motive next matched updates [])
-  (visited : ∀ next matched updates update state stack',
-    state ∈ next →
-    motive next matched updates stack' →
-    motive next matched updates ((update, state) :: stack'))
-  (epsilon : ∀ next matched updates update state stack' state',
-    state ∉ next → nfa[state] = .epsilon state' → motive (next.insert state) matched updates ((update, state') :: stack') →
-    motive next matched updates ((update, state) :: stack'))
-  (split : ∀ next matched updates update state stack' state₁ state₂,
-    state ∉ next → nfa[state] = .split state₁ state₂ →
-    motive (next.insert state) matched updates ((update, state₁) :: (update, state₂) :: stack') →
-    motive next matched updates ((update, state) :: stack'))
-  (save : ∀ next matched updates update state stack' offset state',
-    state ∉ next → nfa[state] = .save offset state' →
-    motive (next.insert state) matched updates ((update ++ [(offset, it.pos)], state') :: stack') →
-    motive next matched updates ((update, state) :: stack'))
-  (done : ∀ next matched updates update state stack',
-    state ∉ next → nfa[state] = .done →
-    motive (next.insert state) (matched <|> some update) (updates.set state state.isLt update) stack' →
-    motive next matched updates ((update, state) :: stack'))
-  (char : ∀ next matched updates update state stack' c state',
-    state ∉ next → nfa[state] = .char c state' →
-    motive (next.insert state) matched (updates.set state state.isLt update) stack' →
-    motive next matched updates ((update, state) :: stack'))
-  (sparse : ∀ next matched updates update state stack' cs state',
-    state ∉ next → nfa[state] = .sparse cs state' →
-    motive (next.insert state) matched (updates.set state state.isLt update) stack' →
-    motive next matched updates ((update, state) :: stack'))
-  (fail : ∀ next matched updates update state stack',
-    state ∉ next → nfa[state] = .fail →
-    motive (next.insert state) matched updates stack' →
-    motive next matched updates ((update, state) :: stack')) :
-  ∀ next matched updates stack, motive next matched updates stack := by
-  refine εClosure'.induct nfa wf it motive base visited ?epsilon ?split ?save ?done ?char ?sparse ?fail
-  case epsilon =>
-    intro next matched updates update state stack' hmem next' state' hn isLt ih
-    exact epsilon next matched updates update state stack' ⟨state', isLt⟩ hmem hn ih
-  case split =>
-    intro next matched updates update state stack' hmem next' state₁ state₂ hn isLt ih
-    exact split next matched updates update state stack' ⟨state₁, isLt.1⟩ ⟨state₂, isLt.2⟩ hmem hn ih
-  case save =>
-    intro next matched updates update state stack' hmem next' offset state' hn isLt update' ih
-    exact save next matched updates update state stack' offset ⟨state', isLt⟩ hmem hn ih
-  case done =>
-    intro next matched updates update state stack' hmem next' hn update' buffer' ih
-    exact done next matched updates update state stack' hmem hn ih
-  case char =>
-    intro next matched updates update state stack' hmem next' c state' hn update' ih
-    exact char next matched updates update state stack' c state' hmem hn ih
-  case sparse =>
-    intro next matched updates update state stack' hmem next' cs state' hn update' ih
-    exact sparse next matched updates update state stack' cs state' hmem hn ih
-  case fail =>
-    intro next matched updates update state stack' hmem next' hn ih
-    exact fail next matched updates update state stack' hmem hn ih
+  (motive : Option (List (Nat × Pos)) → SearchState' nfa → εStack' nfa → Prop)
+  (base : ∀ matched next, motive matched next [])
+  (visited :
+    ∀ matched next update state stack',
+    state ∈ next.states →
+    motive matched next stack' →
+    motive matched next ((update, state) :: stack'))
+  (epsilon : ∀ matched next update state stack' state',
+    state ∉ next.states → nfa[state] = .epsilon state' →
+    let next' := ⟨next.states.insert state, next.updates⟩;
+    motive matched next' ((update, state') :: stack') →
+    motive matched next ((update, state) :: stack'))
+  (split : ∀ matched next update state stack' state₁ state₂,
+    state ∉ next.states → nfa[state] = .split state₁ state₂ →
+    let next' := ⟨next.states.insert state, next.updates⟩;
+    motive matched next' ((update, state₁) :: (update, state₂) :: stack') →
+    motive matched next ((update, state) :: stack'))
+  (save : ∀ matched next update state stack' offset state',
+    state ∉ next.states → nfa[state] = .save offset state' →
+    let next' := ⟨next.states.insert state, next.updates⟩;
+    motive matched next' ((update ++ [(offset, it.pos)], state') :: stack') →
+    motive matched next ((update, state) :: stack'))
+  (done : ∀ matched next update state stack',
+    state ∉ next.states → nfa[state] = .done →
+    let next' := ⟨next.states.insert state, next.updates.set state state.isLt update⟩;
+    motive (matched <|> .some update) next' stack' →
+    motive matched next ((update, state) :: stack'))
+  (char : ∀ matched next update state stack' c (state' : Fin nfa.nodes.size),
+    state ∉ next.states → nfa[state] = .char c state' →
+    let next' := ⟨next.states.insert state, next.updates.set state state.isLt update⟩;
+    motive matched next' stack' →
+    motive matched next ((update, state) :: stack'))
+  (sparse : ∀ matched next update state stack' cs (state' : Fin nfa.nodes.size),
+    state ∉ next.states → nfa[state] = .sparse cs state' →
+    let next' := ⟨next.states.insert state, next.updates.set state state.isLt update⟩;
+    motive matched next' stack' →
+    motive matched next ((update, state) :: stack'))
+  (fail : ∀ matched next update state stack',
+    state ∉ next.states → nfa[state] = .fail →
+    let next' := ⟨next.states.insert state, next.updates⟩;
+    motive matched next' stack' →
+    motive matched next ((update, state) :: stack')) :
+  ∀ matched next stack, motive matched next stack := fun matched next stack =>
+    εClosure'.induct nfa wf it motive base visited
+      (fun matched next update state stack' mem state' hn isLt ih =>
+        epsilon matched next update state stack' ⟨state', isLt⟩ mem hn ih)
+      (fun matched next update state stack' mem state₁ state₂ hn isLt ih =>
+        split matched next update state stack' ⟨state₁, isLt.1⟩ ⟨state₂, isLt.2⟩ mem hn ih)
+      (fun matched next update state stack' mem offset state' hn isLt ih =>
+        save matched next update state stack' offset ⟨state', isLt⟩ mem hn ih)
+      (fun matched next update state stack' mem hn ih =>
+        done matched next update state stack' mem hn ih)
+      (fun matched next update state stack' mem c state' hn ih =>
+        char matched next update state stack' c ⟨state', wf.inBounds' state hn⟩ mem hn ih)
+      (fun matched next update state stack' mem cs state' hn ih =>
+        sparse matched next update state stack' cs ⟨state', wf.inBounds' state hn⟩ mem hn ih)
+      (fun matched next update state stack' mem hn ih =>
+        fail matched next update state stack' mem hn ih)
+      matched next stack
 
 /-
 Simplification lemmas for `εClosure'`.
 -/
 section
 
-variable {nfa wf it next matched updates}
+variable {nfa wf it matched next}
 
 @[simp]
-theorem εClosure'_base : εClosure' nfa wf it next matched updates [] = (next, matched, updates) := by
+theorem εClosure'_base : εClosure' nfa wf it matched next [] = (matched, next) := by
   simp [εClosure']
 
 @[simp]
-theorem εClosure'_visited {update state stack'} (hmem : state ∈ next) :
-  εClosure' nfa wf it next matched updates ((update, state) :: stack') = εClosure' nfa wf it next matched updates stack' := by
+theorem εClosure'_visited {update state stack'} (hmem : state ∈ next.states) :
+  εClosure' nfa wf it matched next ((update, state) :: stack') =
+  εClosure' nfa wf it matched next stack' := by
   simp [εClosure', hmem]
 
 @[simp]
-theorem εClosure'_epsilon {update state stack' state'} (hmem : state ∉ next) (hn : nfa[state] = .epsilon state') :
-  εClosure' nfa wf it next matched updates ((update, state) :: stack') = εClosure' nfa wf it (next.insert state) matched updates ((update, state') :: stack') := by
+theorem εClosure'_epsilon {update state stack' state'} (hmem : state ∉ next.states) (hn : nfa[state] = .epsilon state') :
+  εClosure' nfa wf it matched next ((update, state) :: stack') =
+  εClosure' nfa wf it matched ⟨next.states.insert state, next.updates⟩ ((update, state') :: stack') := by
   conv =>
     lhs
     unfold εClosure'
@@ -140,8 +146,9 @@ theorem εClosure'_epsilon {update state stack' state'} (hmem : state ∉ next) 
   split <;> simp_all
 
 @[simp]
-theorem εClosure'_split {update state stack' state₁ state₂} (hmem : state ∉ next) (hn : nfa[state] = .split state₁ state₂) :
-  εClosure' nfa wf it next matched updates ((update, state) :: stack') = εClosure' nfa wf it (next.insert state) matched updates ((update, state₁) :: (update, state₂) :: stack') := by
+theorem εClosure'_split {update state stack' state₁ state₂} (hmem : state ∉ next.states) (hn : nfa[state] = .split state₁ state₂) :
+  εClosure' nfa wf it matched next ((update, state) :: stack') =
+  εClosure' nfa wf it matched ⟨next.states.insert state, next.updates⟩ ((update, state₁) :: (update, state₂) :: stack') := by
   conv =>
     lhs
     unfold εClosure'
@@ -149,8 +156,9 @@ theorem εClosure'_split {update state stack' state₁ state₂} (hmem : state �
   split <;> simp_all
 
 @[simp]
-theorem εClosure'_save {update state stack' offset state'} (hmem : state ∉ next) (hn : nfa[state] = .save offset state') :
-  εClosure' nfa wf it next matched updates ((update, state) :: stack') = εClosure' nfa wf it (next.insert state) matched updates ((update ++ [(offset, it.pos)], state') :: stack') := by
+theorem εClosure'_save {update state stack' offset state'} (hmem : state ∉ next.states) (hn : nfa[state] = .save offset state') :
+  εClosure' nfa wf it matched next ((update, state) :: stack') =
+  εClosure' nfa wf it matched ⟨next.states.insert state, next.updates⟩ ((update ++ [(offset, it.pos)], state') :: stack') := by
   conv =>
     lhs
     unfold εClosure'
@@ -158,8 +166,9 @@ theorem εClosure'_save {update state stack' offset state'} (hmem : state ∉ ne
   split <;> simp_all
 
 @[simp]
-theorem εClosure'_done {update state stack'} (hmem : state ∉ next) (hn : nfa[state] = .done) :
-  εClosure' nfa wf it next matched updates ((update, state) :: stack') = εClosure' nfa wf it (next.insert state) (matched <|> some update) (updates.set state state.isLt update) stack' := by
+theorem εClosure'_done {update state stack'} (hmem : state ∉ next.states) (hn : nfa[state] = .done) :
+  εClosure' nfa wf it matched next ((update, state) :: stack') =
+  εClosure' nfa wf it (matched <|> .some update) ⟨next.states.insert state, next.updates.set state state.isLt update⟩ stack' := by
   conv =>
     lhs
     unfold εClosure'
@@ -167,8 +176,9 @@ theorem εClosure'_done {update state stack'} (hmem : state ∉ next) (hn : nfa[
   split <;> simp_all
 
 @[simp]
-theorem εClosure'_char {update state stack' c state'} (hmem : state ∉ next) (hn : nfa[state] = .char c state') :
-  εClosure' nfa wf it next matched updates ((update, state) :: stack') = εClosure' nfa wf it (next.insert state) matched (updates.set state state.isLt update) stack' := by
+theorem εClosure'_char {update state stack' c state'} (hmem : state ∉ next.states) (hn : nfa[state] = .char c state') :
+  εClosure' nfa wf it matched next ((update, state) :: stack') =
+  εClosure' nfa wf it matched ⟨next.states.insert state, next.updates.set state state.isLt update⟩ stack' := by
   conv =>
     lhs
     unfold εClosure'
@@ -176,8 +186,9 @@ theorem εClosure'_char {update state stack' c state'} (hmem : state ∉ next) (
   split <;> simp_all
 
 @[simp]
-theorem εClosure'_sparse {update state stack' cs state'} (hmem : state ∉ next) (hn : nfa[state] = .sparse cs state') :
-  εClosure' nfa wf it next matched updates ((update, state) :: stack') = εClosure' nfa wf it (next.insert state) matched (updates.set state state.isLt update) stack' := by
+theorem εClosure'_sparse {update state stack' cs state'} (hmem : state ∉ next.states) (hn : nfa[state] = .sparse cs state') :
+  εClosure' nfa wf it matched next ((update, state) :: stack') =
+  εClosure' nfa wf it matched ⟨next.states.insert state, next.updates.set state state.isLt update⟩ stack' := by
   conv =>
     lhs
     unfold εClosure'
@@ -185,8 +196,9 @@ theorem εClosure'_sparse {update state stack' cs state'} (hmem : state ∉ next
   split <;> simp_all
 
 @[simp]
-theorem εClosure'_fail {update state stack'} (hmem : state ∉ next) (hn : nfa[state] = .fail) :
-  εClosure' nfa wf it next matched updates ((update, state) :: stack') = εClosure' nfa wf it (next.insert state) matched updates stack' := by
+theorem εClosure'_fail {update state stack'} (hmem : state ∉ next.states) (hn : nfa[state] = .fail) :
+  εClosure' nfa wf it matched next ((update, state) :: stack') =
+  εClosure' nfa wf it matched ⟨next.states.insert state, next.updates⟩ stack' := by
   conv =>
     lhs
     unfold εClosure'
